FOL/NV/Prop.lean
@@ -32,9 +32,9 @@ axiom def_iff_ (phi psi : Formula) : iff_ phi psi = (phi.imp_ psi).and_ (psi.imp
 /--
   ∃ x phi := ¬ ∀ x ¬ phi
 -/
-axiom def_exists_ (x : VarName) (phi : Formula) : exists_ x phi = not_ (forall_ x (not_ phi))
+axiom def_exists_ (x : VarName_) (phi : Formula) : exists_ x phi = not_ (forall_ x (not_ phi))
 
-def def_eq_ (x y : VarName) : Formula :=
+def def_eq_ (x y : VarName_) : Formula :=
   pred_const_ (PredName.mk "=") [x, y]
 
 
